theories/L/Complexity/PolyBounds.v
@@ -1,8 +1,8 @@
-From Undecidability.L Require Export Datatypes.Lists.
 
 From Undecidability.L.Complexity Require Export NP ONotation. 
 From Undecidability.L.Tactics Require Import LTactics.
 From Undecidability.L.Complexity Require Import MorePrelim.
+From Undecidability.L Require Export Datatypes.LLists Datatypes.LLNat.
 
 Lemma list_el_size_bound {X : Type} `{registered X} (l : list X) (a : X) :
   a el l -> size(enc a) <= size(enc l). 
@@ -60,6 +60,11 @@ Proof.
   - cbn. rewrite IHl. lia. 
 Qed. 
 
+Lemma list_size_enc_length {X : Type} `{registered X} (l : list X) : size (enc (|l|)) <= size (enc l). 
+Proof. 
+  rewrite size_list. rewrite size_nat_enc. induction l; cbn; lia. 
+Qed. 
+
 Lemma list_size_of_el {X : Type} `{registered X} (l : list X) (k : nat) : (forall a, a el l -> size(enc a) <= k) -> size(enc l) <= (k * (|l|)) + 5 * (|l|) +  4 . 
 Proof.
   intros H1. induction l. 
@@ -69,6 +74,45 @@ Proof.
 Qed. 
 
 
+Tactic Notation "replace_le" constr(s) "with" constr(r) "by" tactic(tac) :=
+  let H := fresh in assert (s <= r) as H by tac; rewrite !H; clear H. 
+Tactic Notation "replace_le" constr(s) "with" constr(r) "by" tactic(tac) "at" integer(occ) := 
+  let H := fresh in assert (s <= r) as H by tac; rewrite H at occ; clear H. 
+
+
+Tactic Notation "poly_mono" constr(H) "at" integer(occ) :=
+  let He := fresh in specialize H as He; match type of He with
+                    | _ /\ monotonic _ => unfold monotonic in He; setoid_rewrite (proj2 He) at occ
+                    | monotonic _ /\ _ => unfold monotonic in He; setoid_rewrite (proj1 He) at occ
+                    end; clear He. 
+Tactic Notation "poly_mono" constr(H) :=
+  let He := fresh in specialize H as He; match type of He with
+                    | _ /\ monotonic _ => unfold monotonic in He; erewrite (proj2 He)
+                    | monotonic _ /\ _ => unfold monotonic in He; erewrite (proj1 He)
+                    end; clear He. 
+
+
+Lemma le_add_l n m : m <= n + m. 
+Proof. lia. Qed. 
+
+Definition c__moduloBound :=  c__divmod + c__modulo.
+Lemma modulo_time_bound x y: 
+  modulo_time x y <= (size (enc x) + size (enc y) + 1) * c__moduloBound. 
+Proof. 
+  unfold modulo_time, divmod_time. rewrite size_nat_enc_r with (n := x) at 1. rewrite size_nat_enc_r with (n := y) at 1.
+  unfold c__moduloBound. nia. 
+Qed. 
+
+Lemma leb_time_bound_l a b: leb_time a b <= (size(enc a) + 1) * c__leb. 
+Proof. 
+  unfold leb_time. rewrite Nat.le_min_l. rewrite size_nat_enc_r with (n := a) at 1. lia.
+Qed. 
+
+Lemma leb_time_bound_r a b : leb_time a b <= (size(enc b) + 1) * c__leb. 
+Proof. 
+  unfold leb_time. rewrite Nat.le_min_r. rewrite size_nat_enc_r with (n:= b) at 1. lia. 
+Qed. 
+
 Section fixX.
   Context {X : Type}.
   Context {H : registered X}.
@@ -77,79 +121,103 @@ Section fixX.
   (* i.e. their running time depends on some values in their environment *)
   Variable (Y : Type).
   Context {RY : registered Y}.
-  Lemma list_in_decb_time_bound_env (eqbT : Y -> timeComplexity (X -> X -> bool)) :
-    (exists (f : nat -> nat), (forall (a b : X) (y : Y), callTime2 (eqbT y) a b <= f(size(enc a) + size(enc b) + size(enc y))) /\ inOPoly f /\ monotonic f)
-      -> exists (f : nat -> nat), (forall (l : list X) (e : X) (y : Y), list_in_decb_time (eqbT y) l e <= f(size(enc l) + size(enc e) + size (enc y))) /\ inOPoly f /\ monotonic f. 
+
+  Lemma list_in_decb_time_bound_env (eqbT : Y -> (X -> X -> nat)) (f : nat -> nat):
+    (forall (a b : X) (y : Y), eqbT y a b <= f(size(enc a) + size(enc b) + size(enc y))) /\ monotonic f 
+      -> forall (l : list X) (e : X) (y : Y), list_in_decb_time (eqbT y) l e <= ((|l| + 1) * (f(size(enc l) + size(enc e) + size(enc y)) + c__list_in_decb)).  
   Proof.
-    intros (f' & H1 & H2 & H3). 
-    evar (f : nat -> nat). exists f; split. 
-    - intros l e y. unfold list_in_decb_time. 
-      (*bound each step *)
-      assert (forall (a : X) (y : Y) (l : list X), a el l -> callTime2 (eqbT y) a e <= f'(size(enc l) + size(enc e) + size(enc y))). 
-      {clear l. intros a y0 l He. rewrite H1. apply H3. rewrite list_el_size_bound. 2: apply He. reflexivity. }
-      (* with a tighter analysis, one could obtain a linear bound, but this is not worth the hassle *)
-      instantiate (f:= fun n => f' n * n + 16 * n + 4). subst f. 
-      induction l. 
-      * solverec. 
-      * rewrite IHl. rewrite H0 with (l:= a::l). clear IHl. 2 : now left.
-        solverec. rewrite list_size_cons at 4. solverec.
-        unfold monotonic in H3; rewrite H3 with (x:= (size (enc l) + size(enc e) + size(enc y))) (x' := size(enc(a::l)) + size(enc e) + size(enc y)). 
-        rewrite list_size_cons. solverec. 
-        rewrite list_size_cons; lia. 
-    - split; unfold f; smpl_inO. 
+    intros [H1 H2]. intros. induction l. 
+    - rewrite size_list; cbn. nia.
+    - cbn [list_in_decb_time]. rewrite IHl, H1. unfold monotonic in H2. 
+      rewrite H2 with (x' := size (enc (a ::l)) + size(enc e) + size(enc y)). 
+      2: rewrite list_size_cons; unfold c__list_in_decb; nia. 
+      setoid_rewrite H2 with (x' := size (enc (a ::l)) + size(enc e) + size(enc y)) at 2. 
+      2: rewrite list_size_cons; unfold c__list_in_decb; nia. 
+      cbn. solverec. 
   Qed. 
 
-  Lemma dupfreeb_time_bound_env (eqbT : Y -> timeComplexity (X -> X -> bool)):
-    (*eqbT is polynomial in encoding of a and b and the environment y *)
-    (exists (f : nat -> nat), (forall (a b : X) (y : Y), callTime2 (eqbT y) a b <= f (size(enc a) + size(enc b) + size(enc y))) /\ inOPoly f /\ monotonic f)
-    -> exists (f : nat -> nat), (forall (l : list X) (y : Y), dupfreeb_time (eqbT y) l <= f (size(enc l) + size(enc y))) /\ inOPoly f /\ monotonic f. 
-  Proof.
-    intros H1.
-    specialize (list_in_decb_time_bound_env H1) as (f_indec & F1 & F2 & F3).
-    destruct H1 as (f' & H1 & H2).  
-    evar (f : nat -> nat). exists f. split; try split.
-    1:{ intros l y. unfold dupfreeb_time.   
-      instantiate (f := fun n => n * f_indec (n) + 25 *n + 8). subst f. 
-      induction l. 
-      + lia. 
-      + rewrite IHl. rewrite F1. clear IHl. solverec. rewrite list_size_cons.
-        unfold monotonic in F3. rewrite F3 with (x' := size(enc a) + size(enc l) +5 + size(enc y)). 2:lia.
-        rewrite F3 with (x := size(enc l) + size(enc y)) (x' := size (enc a) + size(enc l) + 5 + size(enc y)). solverec. lia. 
-      }
-    all: subst f; smpl_inO.  
-  Qed. 
+  (*
+     TODO:two possible approaches for higher order functions
+              - either conditional polynomial: but has the problem that one needs lazier overapproximations which evokes difficulties with nia etc
+              - tighter bounds that are non-compositional: see higher order functions as a template, their running time bounds do not tell the fulls story -> need to restate parts of the functions if it is used by another higher-order functin
 
-  Lemma forallb_time_bound_env (predT : Y -> timeComplexity(X -> bool)) :
-    (exists (f : nat -> nat), (forall (a : X) (y : Y), fst(predT y a tt) <= f (size(enc a) + size(enc y))) /\ inOPoly f /\ monotonic f)
-    -> exists (f : nat -> nat), (forall (l : list X) (y : Y), forallb_time (predT y) l <= f(size (enc l) + size(enc y)) ) /\ inOPoly f /\ monotonic f. 
+   *)
+
+  (* Lemma dupfreeb_time_bound_env (eqbT : Y -> X -> X -> nat) (f : nat -> nat): *)
+  (*   (forall (a b : X) (y : Y), eqbT y a b <= f (size (enc a) + size (enc b) + size(enc y))) /\ monotonic f *)
+  (*    -> forall (l : list X) (y : Y), dupfreeb_time (eqbT y) l <= (|l| + 1) * (f (size (enc l) + size (enc y)) + c__dupfreeb).  *)
+  (* Proof.  *)
+  (*   intros [H1 H2]. intros. induction l.  *)
+  (*   - cbn. lia.  *)
+  (*   - cbn. rewrite IHl. rewrite list_in_decb_time_bound_env by easy.   *)
+  (*     unfold monotonic in H2. erewrite H2. *)
+  (*     2: (replace_le (size (enc l) + size (enc a)) with (size (enc (a::l))) by (rewrite list_size_cons; lia)); reflexivity. *)
+  (*     setoid_rewrite H2 at 2.  *)
+  (*     2: (replace_le (size(enc l)) with (size (enc (a::l))) by (rewrite list_size_cons; lia)); reflexivity. *)
+  (*     nia.  *)
+
+  (* Lemma dupfreeb_time_bound_env (eqbT : Y -> X -> X -> nat): *)
+  (*   (* eqbT is polynomial in encoding of a and b and the environment y *) *)
+  (*   (exists (f : nat -> nat), (forall (a b : X) (y : Y), eqbT y a b <= f (size(enc a) + size(enc b) + size(enc y))) /\ inOPoly f /\ monotonic f) *)
+  (*   -> exists (f : nat -> nat), (forall (l : list X) (y : Y), dupfreeb_time (eqbT y) l <= f (size(enc l) + size(enc y))) /\ inOPoly f /\ monotonic f. *)
+  (* Proof. *)
+  (*   intros H1. *)
+  (*   specialize (list_in_decb_time_bound_env H1) as (f_indec & F1 & F2 & F3). *)
+  (*   destruct H1 as (f' & H1 & H2). *)
+  (*   evar (f : nat -> nat). exists f. split; try split. *)
+  (*   1:{ intros l y. unfold dupfreeb_time. *)
+  (*     instantiate (f := fun n => n * f_indec (n) + c__dupfreeb *n + c__dupfreeb). subst f. *)
+  (*     induction l. *)
+  (*     + lia. *)
+  (*     + rewrite IHl. rewrite F1. clear IHl. solverec. rewrite list_size_cons. *)
+  (*       unfold monotonic in F3. rewrite F3 with (x' := size(enc a) + size(enc l) +5 + size(enc y)). 2:lia. *)
+  (*       rewrite F3 with (x := size(enc l) + size(enc y)) (x' := size (enc a) + size(enc l) + 5 + size(enc y)). solverec. lia. *)
+  (*     } *)
+  (*   all: subst f; smpl_inO. *)
+  (* Qed. *)
+
+  Lemma forallb_time_bound_env (predT : Y -> X -> nat) (f : nat -> nat):
+    (forall (a : X) (y : Y), predT y a <= f (size(enc a) + size(enc y))) /\ monotonic f 
+    -> forall (l : list X) (y : Y), forallb_time (predT y) l <= (|l| +1) * (f(size (enc l) + size(enc y)) + c__forallb). 
   Proof. 
-    intros (f' & H1 & H2 & H3). 
-    evar (f : nat -> nat). exists f. split; try split.
-    1: {
-      intros l y. unfold forallb_time.
-      assert (forall (a : X) (l : list X) (y : Y), a el l -> fst(predT y a tt) <= f'(size (enc l) + size(enc y))).
-      { clear l. intros a l y0 H4. rewrite H1. unfold monotonic in H3; rewrite H3.
-        2: { enough (size(enc a) + size(enc y0) <= size(enc l) + size (enc y0)) by apply H0. now rewrite list_el_size_bound. }
-        lia. }
-      instantiate (f := fun n => n * f' n + 15 * n + 8). subst f.
-      induction l. 
-      - cbn; lia. 
-      - cbn -[ Nat.mul]. rewrite IHl. rewrite H0. 2: {assert (a el a :: l) by firstorder. apply H4. }
-      rewrite list_size_cons at 2. unfold monotonic in H3; rewrite H3 with (x:= size(enc l) + size(enc y)) (x' := size(enc(a::l)) + size(enc y)).  
-      rewrite list_size_cons at 4. solverec. 
-      rewrite list_size_cons; lia. 
-    }
-    all: unfold f; smpl_inO. 
+    intros [H1 H2]. intros. induction l. 
+    - cbn. lia.   
+    - cbn. rewrite IHl, H1. unfold monotonic in H2. 
+      rewrite H2 with (x' := size (enc (a :: l)) + size(enc y)). 2: rewrite list_size_cons; nia. 
+      setoid_rewrite H2 with (x' := size(enc (a::l)) + size(enc y)) at 2. 2: rewrite list_size_cons; nia. 
+      nia.
   Qed. 
 
-  Lemma nth_error_time_bound : exists (f : nat -> nat), (forall (l : list X) (n : nat), callTime2 (@nth_error_time X) l n <= f(size (enc l))) /\ inOPoly f /\ monotonic f. 
+  (*Lemma forallb_time_bound_env (predT : Y -> X -> nat) :*)
+    (*(exists (f : nat -> nat), (forall (a : X) (y : Y), predT y a <= f (size(enc a) + size(enc y))) /\ inOPoly f /\ monotonic f)*)
+    (*-> exists (f : nat -> nat), (forall (l : list X) (y : Y), forallb_time (predT y) l <= f(size (enc l) + size(enc y)) ) /\ inOPoly f /\ monotonic f. *)
+  (*Proof. *)
+    (*intros (f' & H1 & H2 & H3). *)
+    (*evar (f : nat -> nat). exists f. split; try split.*)
+    (*1: {*)
+      (*intros l y. unfold forallb_time.*)
+      (*assert (forall (a : X) (l : list X) (y : Y), a el l -> predT y a <= f'(size (enc l) + size(enc y))).*)
+      (*{ clear l. intros a l y0 H4. rewrite H1. unfold monotonic in H3; rewrite H3.*)
+        (*2: { enough (size(enc a) + size(enc y0) <= size(enc l) + size (enc y0)) by apply H0. now rewrite list_el_size_bound. }*)
+        (*lia. }*)
+      (*instantiate (f := fun n => n * f' n + c__forallb * n + c__forallb). subst f.*)
+      (*induction l. *)
+      (*- cbn; lia. *)
+      (*- cbn -[ Nat.mul]. rewrite IHl. rewrite H0. 2: {assert (a el a :: l) by firstorder. apply H4. }*)
+      (*rewrite list_size_cons at 2. unfold monotonic in H3; rewrite H3 with (x:= size(enc l) + size(enc y)) (x' := size(enc(a::l)) + size(enc y)).  *)
+      (*rewrite list_size_cons at 4. solverec. *)
+      (*rewrite list_size_cons; lia. *)
+    (*}*)
+    (*all: unfold f; smpl_inO. *)
+  (*Qed. *)
+
+  Lemma nth_error_time_bound : exists (f : nat -> nat), (forall (l : list X) (n : nat), nth_error_time l <= f(size (enc l))) /\ inOPoly f /\ monotonic f. 
   Proof.
     evar (f : nat -> nat). exists f. split.
-    - intros. unfold nth_error_time. cbn -[Nat.add Nat.mul]. rewrite Nat.le_min_r. specialize (list_size_length l). 
-      instantiate (f := fun n => 15 + 15 * n). subst f. solverec. 
+    - intros. unfold nth_error_time. specialize (list_size_length l). 
+      instantiate (f := fun n => (c__ntherror) * (1 + n)). subst f. solverec. nia.
     - subst f; split; smpl_inO. 
   Qed. 
-
 End fixX.
 
 Section fixXY.
@@ -161,41 +229,42 @@ Section fixXY.
   (*the running time of foldr not only depends on the running time of the step function, *)
   (*but also on the output size of the step function; in order to get a polynomial bound, *)
   (*we require that this output size grows only by an additive constant in each step *)
-  Lemma fold_right_time_bound_env (step : Z -> Y -> X -> X) (stepT : Z -> timeComplexity (Y -> X -> X)) :
-    (exists (f : nat -> nat), (forall (acc : X) (ele : Y) (env : Z), callTime2 (stepT env) ele acc <= f(size(enc acc) + size(enc ele) + size(enc env))) /\ inOPoly f /\ monotonic f)
-    -> (exists (c__out c__out' : nat), forall (acc : X) (ele : Y) (env : Z), size(enc (step env ele acc)) <= size(enc acc) + c__out' * (size(enc ele) + size(enc env)) + c__out)
+  Lemma fold_right_time_bound_env (step : Z -> Y -> X -> X) (stepT : Z -> (Y -> X -> nat)) :
+    (exists (f : nat -> nat), (forall (acc : X) (ele : Y) (env : Z), stepT env ele acc <= f(size(enc acc) + size(enc ele) + size(enc env))) /\ inOPoly f /\ monotonic f)
+    -> (exists (f_size :nat -> nat), (forall (acc : X) (ele : Y) (env : Z), size(enc (step env ele acc)) <= size(enc acc) + f_size (size(enc ele) + size(enc env))) /\ inOPoly f_size /\ monotonic f_size)
     -> exists (f : nat -> nat), (forall (l : list Y) (acc : X) (env : Z), fold_right_time (step env) (stepT env) l acc <= f(size(enc l) + size(enc acc) + size(enc env))) /\ inOPoly f /\ monotonic f.
   Proof.
-    intros (f__step & H2 & H3 & H4) (c__out & c__out' & F). 
-    evar (f : nat -> nat). exists f. split.
-    - intros l init env.
-      (* we first show that the output size of foldr on every suffix is polynomial *)
-      assert (forall l' l'', l = l' ++ l'' -> size(enc (fold_right (step env) init l'')) <= size(enc init) + c__out' * size(enc l'') + (|l''|) * (c__out' * size(enc env) + c__out)).
-      {
-        intros l' l''; revert l'. induction l''.
-        + cbn. intros; lia.
-        + intros. cbn. rewrite F. rewrite IHl''. 2: { now rewrite app_comm_cons' in H5. }
-          rewrite list_size_cons. solverec. 
-      }
+(*    intros (f__step & H2 & H3 & H4) (f_size & F1 & F2 & F3). *)
+    (*evar (f : nat -> nat). exists f. split.*)
+    (*- intros l init env.*)
+      (*[> we first show that the output size of foldr on every suffix is polynomial <]*)
+      (*assert (forall l' l'', l = l' ++ l'' -> size(enc (fold_right (step env) init l'')) <= size(enc init) + c__out' * size(enc l'') + (|l''|) * (c__out' * size(enc env) + c__out)).*)
+      (*{*)
+        (*intros l' l''; revert l'. induction l''.*)
+        (*+ cbn. intros; lia.*)
+        (*+ intros. cbn. rewrite F. rewrite IHl''. 2: { now rewrite app_comm_cons' in H5. }*)
+          (*rewrite list_size_cons. solverec. *)
+      (*}*)
 
-      instantiate (f := fun n => 4 + n * f__step((S c__out) * (S c__out') * n * n + (S c__out') * n) + 15 * n). subst f.
-      unfold fold_right_time. 
-      induction l.
-      + solverec.
-      + rewrite IHl, H2.
-        * unfold monotonic in H4.
-          rewrite H4 with (x' := (S c__out) * (S c__out') * (size(enc(a::l)) + size(enc init) + size(enc env)) *  (size(enc(a::l)) + size(enc init) + size(enc env)) + (S c__out') * (size(enc(a::l)) + size(enc init) + size(enc env))). 
-          2: {clear IHl. rewrite H5. rewrite list_size_length. rewrite list_size_cons.
-              2: {assert (a::l = [a] ++ l) as H6 by reflexivity; apply H6. }
-              cbn. rewrite Nat.mul_add_distr_l. nia. }
+      (*instantiate (f := fun n => 4 + n * f__step((S c__out) * (S c__out') * n * n + (S c__out') * n) + 15 * n). subst f.*)
+      (*unfold fold_right_time. *)
+      (*induction l.*)
+      (*+ solverec.*)
+      (*+ rewrite IHl, H2.*)
+        (** unfold monotonic in H4.*)
+          (*rewrite H4 with (x' := (S c__out) * (S c__out') * (size(enc(a::l)) + size(enc init) + size(enc env)) *  (size(enc(a::l)) + size(enc init) + size(enc env)) + (S c__out') * (size(enc(a::l)) + size(enc init) + size(enc env))). *)
+          (*2: {clear IHl. rewrite H5. rewrite list_size_length. rewrite list_size_cons.*)
+              (*2: {assert (a::l = [a] ++ l) as H6 by reflexivity; apply H6. }*)
+              (*cbn. rewrite Nat.mul_add_distr_l. nia. }*)
 
-          setoid_rewrite H4 with (x' := (S c__out) * (S c__out') * (size(enc(a::l)) + size(enc init) + size(enc env)) *  (size(enc(a::l)) + size(enc init) + size(enc env)) + (S c__out') * (size(enc(a::l)) + size(enc init) + size(enc env))) at 2. 
-          2: {clear IHl. rewrite list_size_cons. cbn; nia. }
+          (*setoid_rewrite H4 with (x' := (S c__out) * (S c__out') * (size(enc(a::l)) + size(enc init) + size(enc env)) *  (size(enc(a::l)) + size(enc init) + size(enc env)) + (S c__out') * (size(enc(a::l)) + size(enc init) + size(enc env))) at 2. *)
+          (*2: {clear IHl. rewrite list_size_cons. cbn; nia. }*)
 
-          rewrite list_size_cons at 7. rewrite list_size_cons at 10. solverec. 
-       * clear IHl. intros. apply H5 with (l' := a::l'). firstorder. 
-    - subst f; split; smpl_inO. apply inOPoly_comp; smpl_inO. 
-  Qed. 
+          (*rewrite list_size_cons at 7. rewrite list_size_cons at 10. solverec. *)
+       (** clear IHl. intros. apply H5 with (l' := a::l'). firstorder. *)
+    (*- subst f; split; smpl_inO. apply inOPoly_comp; smpl_inO. *)
+(*  Qed. *)
+  Admitted. 
 End fixXY.
 
 
@@ -204,82 +273,81 @@ Require Import Undecidability.L.Datatypes.LUnit.
 Section noEnv.
   Context {X : Type}.
   Context {H : registered X}.
-  Lemma list_in_decb_time_bound (eqbT : timeComplexity (X -> X -> bool)) :
-    (exists (f : nat -> nat), (forall (a b : X), callTime2 eqbT a b <= f(size(enc a) + size(enc b))) /\ inOPoly f /\ monotonic f)
-      -> exists (f : nat -> nat), (forall (l : list X) (e : X), list_in_decb_time eqbT l e <= f(size(enc l) + size(enc e))) /\ inOPoly f /\ monotonic f. 
-  Proof.
-    intros (f' & H1 & H2 & H3). 
-    assert (exists (f' : nat -> nat), (forall (a b : X) (y : unit), callTime2 eqbT a b <= f'(size(enc a) + size(enc b) + size(enc y))) /\ inOPoly f' /\ monotonic f').
-    { exists f'. split.
-      + intros a b y. rewrite H1. unfold monotonic in H3. apply H3. lia.
-      + tauto. 
-    }
-    specialize (list_in_decb_time_bound_env H0) as (f & F1 & F2 & F3). 
-    exists (fun n => f (n + 2)). (* Compute (size (enc tt)) evaluates to 2*)
-    split. 
-    + intros. rewrite <- size_unit_enc. apply F1. 
-    + split; smpl_inO. apply inOPoly_comp; smpl_inO. 
-  Qed. 
+  (*Lemma list_in_decb_time_bound (eqbT : X -> X -> nat) :*)
+    (*(exists (f : nat -> nat), (forall (a b : X), eqbT a b <= f(size(enc a) + size(enc b))) /\ inOPoly f /\ monotonic f)*)
+      (*-> exists (f : nat -> nat), (forall (l : list X) (e : X), list_in_decb_time eqbT l e <= f(size(enc l) + size(enc e))) /\ inOPoly f /\ monotonic f. *)
+  (*Proof.*)
+    (*intros (f' & H1 & H2 & H3). *)
+    (*assert (exists (f' : nat -> nat), (forall (a b : X) (y : unit), eqbT a b <= f'(size(enc a) + size(enc b) + size(enc y))) /\ inOPoly f' /\ monotonic f').*)
+    (*{ exists f'. split.*)
+      (*+ intros a b y. rewrite H1. unfold monotonic in H3. apply H3. lia.*)
+      (*+ tauto. *)
+    (*}*)
+    (*specialize (list_in_decb_time_bound_env H0) as (f & F1 & F2 & F3). *)
+    (*exists (fun n => f (n + 2)). [> Compute (size (enc tt)) evaluates to 2<]*)
+    (*split. *)
+    (*+ intros. rewrite <- size_unit_enc. apply F1. *)
+    (*+ split; smpl_inO. apply inOPoly_comp; smpl_inO. *)
+  (*Qed. *)
 
-  Lemma dupfreeb_time_bound (eqbT : timeComplexity (X -> X -> bool)):
-    (exists (f : nat -> nat), (forall (a b : X), callTime2 eqbT a b <= f (size(enc a) + size(enc b))) /\ inOPoly f /\ monotonic f)
-    -> exists (f : nat -> nat), (forall (l : list X), dupfreeb_time eqbT l <= f (size(enc l))) /\ inOPoly f /\ monotonic f. 
-  Proof.
-    intros (f' & H1 & H2 & H3).
-    assert (exists (f' : nat -> nat),(forall (a b : X) (y : unit), callTime2 eqbT a b <= f' (size(enc a) + size(enc b) + size(enc y))) /\ inOPoly f' /\ monotonic f').
-    { exists f'; split.
-      - intros; rewrite H1. unfold monotonic in H3. apply H3. lia.
-      - tauto.
-    }
-    specialize (dupfreeb_time_bound_env H0) as (f & F1 & F2 & F3). 
-    exists (fun n => f (n + 2)). (* Compute (size (enc tt)) evaluates to 2*)
-    split. 
-    + intros. now rewrite <- size_unit_enc.
-    + split; smpl_inO. apply inOPoly_comp; smpl_inO. 
-  Qed. 
+  (*Lemma dupfreeb_time_bound (eqbT : X -> X -> nat):*)
+    (*(exists (f : nat -> nat), (forall (a b : X), eqbT a b <= f (size(enc a) + size(enc b))) /\ inOPoly f /\ monotonic f)*)
+    (*-> exists (f : nat -> nat), (forall (l : list X), dupfreeb_time eqbT l <= f (size(enc l))) /\ inOPoly f /\ monotonic f. *)
+  (*Proof.*)
+    (*intros (f' & H1 & H2 & H3).*)
+    (*assert (exists (f' : nat -> nat),(forall (a b : X) (y : unit), eqbT a b <= f' (size(enc a) + size(enc b) + size(enc y))) /\ inOPoly f' /\ monotonic f').*)
+    (*{ exists f'; split.*)
+      (*- intros; rewrite H1. unfold monotonic in H3. apply H3. lia.*)
+      (*- tauto.*)
+    (*}*)
+    (*specialize (dupfreeb_time_bound_env H0) as (f & F1 & F2 & F3). *)
+    (*exists (fun n => f (n + 2)). [> Compute (size (enc tt)) evaluates to 2<]*)
+    (*split. *)
+    (*+ intros. now rewrite <- size_unit_enc.*)
+    (*+ split; smpl_inO. apply inOPoly_comp; smpl_inO. *)
+  (*Qed. *)
 
-  Lemma forallb_time_bound (predT : timeComplexity(X -> bool)) :
-    (exists (f : nat -> nat), (forall (a : X),  fst(predT a tt) <= f (size(enc a))) /\ inOPoly f /\ monotonic f)
-    -> exists (f : nat -> nat), (forall (l : list X), forallb_time predT l <= f(size (enc l))) /\ inOPoly f /\ monotonic f.
-  Proof. 
-    intros (f' & H1 & H2 & H3).
-    assert (exists (f' : nat -> nat),(forall (a : X) (y : unit), fst((fun (_ : unit) a (b : unit) => predT a b) y a tt) <= f' (size(enc a) + size(enc y))) /\ inOPoly f' /\ monotonic f').
-    { exists f'; split.
-      - intros; rewrite H1. unfold monotonic in H3. apply H3. lia.
-      - tauto.
-    }
-    specialize (forallb_time_bound_env H0) as (f & F1 & F2 & F3). 
-    exists (fun n => f (n + 2)). (* Compute (size (enc tt)) evaluates to 2*)
-    split. 
-    + intros. now rewrite <- size_unit_enc.
-    + split; smpl_inO. apply inOPoly_comp; smpl_inO. 
-  Qed. 
+  (*Lemma forallb_time_bound (predT : X -> nat) :*)
+    (*(exists (f : nat -> nat), (forall (a : X),  predT a  <= f (size(enc a))) /\ inOPoly f /\ monotonic f)*)
+    (*-> exists (f : nat -> nat), (forall (l : list X), forallb_time predT l <= f(size (enc l))) /\ inOPoly f /\ monotonic f.*)
+  (*Proof. *)
+    (*intros (f' & H1 & H2 & H3).*)
+    (*assert (exists (f' : nat -> nat),(forall (a : X) (y : unit), (fun (_ : unit) a=> predT a) y a <= f' (size(enc a) + size(enc y))) /\ inOPoly f' /\ monotonic f').*)
+    (*{ exists f'; split.*)
+      (*- intros; rewrite H1. unfold monotonic in H3. apply H3. lia.*)
+      (*- tauto.*)
+    (*}*)
+    (*specialize (forallb_time_bound_env H0) as (f & F1 & F2 & F3). *)
+    (*exists (fun n => f (n + 2)). [> Compute (size (enc tt)) evaluates to 2<]*)
+    (*split. *)
+    (*+ intros. now rewrite <- size_unit_enc.*)
+    (*+ split; smpl_inO. apply inOPoly_comp; smpl_inO. *)
+  (*Qed. *)
 
-  Variable (Y : Type).
-  Context {H0 : registered Y}. 
-  Lemma fold_right_time_bound (step : Y -> X -> X) (stepT : timeComplexity (Y -> X -> X)) :
-    (exists (f : nat -> nat), (forall (acc : X) (ele : Y), callTime2 stepT ele acc <= f(size(enc acc) + size(enc ele))) /\ inOPoly f /\ monotonic f)
-    -> (exists (c__out c__out' : nat), forall (acc : X) (ele : Y), size(enc (step ele acc)) <= size(enc acc) + c__out' * size(enc ele) + c__out)
-    -> exists (f : nat -> nat), (forall (l : list Y) (acc : X), fold_right_time step stepT l acc <= f(size(enc l) + size(enc acc))) /\ inOPoly f /\ monotonic f.
-  Proof.
-    intros (f' & H1 & H2 & H3).
-    intros (c__out & c__out' & F). 
-    assert (exists (f : nat -> nat), (forall (acc : X) (ele : Y) (env : unit), callTime2 stepT ele acc <= f(size(enc acc) + size(enc ele) + size(enc env))) /\ inOPoly f /\ monotonic f). 
-    {
-      exists f'; split. 
-      - intros; rewrite H1. unfold monotonic in H3. apply H3. lia. 
-      - split; smpl_inO. 
-    }
-    assert (exists (c__out c__out': nat), forall (acc : X) (ele : Y) (env : unit), size(enc (step ele acc)) <= size(enc acc) + c__out' * (size(enc ele) + size(enc env)) + c__out).
-    {
-      exists c__out, c__out'. intros. rewrite F. nia. 
-    }
-    specialize (fold_right_time_bound_env H4 H5) as (f & G1 & G2 & G3).
-    exists (fun n => f (n + 2)). 
-    split.
-    - intros. rewrite G1 with (env := tt). now rewrite <- size_unit_enc. 
-    - split; smpl_inO. apply inOPoly_comp; smpl_inO. 
-  Qed. 
-
+  (*Variable (Y : Type).*)
+  (*Context {H0 : registered Y}. *)
+  (*Lemma fold_right_time_bound (step : Y -> X -> X) (stepT : Y -> X -> nat) :*)
+    (*(exists (f : nat -> nat), (forall (acc : X) (ele : Y), stepT ele acc <= f(size(enc acc) + size(enc ele))) /\ inOPoly f /\ monotonic f)*)
+    (*-> (exists (f_size : nat -> nat), (forall (acc : X) (ele : Y), size(enc (step ele acc)) <= size(enc acc) + f_size(size(enc ele))) /\ inOPoly f_size /\ monotonic f_size)*)
+    (*-> exists (f : nat -> nat), (forall (l : list Y) (acc : X), fold_right_time step stepT l acc <= f(size(enc l) + size(enc acc))) /\ inOPoly f /\ monotonic f.*)
+  (*Proof.*)
+    (*intros (f' & H1 & H2 & H3).*)
+    (*intros (f_size & F1 & F2 & F3). *)
+    (*assert (exists (f : nat -> nat), (forall (acc : X) (ele : Y) (env : unit), stepT ele acc <= f(size(enc acc) + size(enc ele) + size(enc env))) /\ inOPoly f /\ monotonic f). *)
+    (*{*)
+      (*exists f'; split. *)
+      (*- intros; rewrite H1. unfold monotonic in H3. apply H3. lia. *)
+      (*- split; smpl_inO. *)
+    (*}*)
+    (*assert (exists (f_size: nat->nat), (forall (acc : X) (ele : Y) (env : unit), size(enc (step ele acc)) <= size(enc acc) + f_size((size(enc ele) + size(enc env)))) /\ inOPoly f_size /\ monotonic f_size).*)
+    (*{*)
+      (*exists f_size. split; [ | easy]. intros. rewrite F1. unfold monotonic in F3. rewrite F3 with (x' := size(enc ele) + size(enc env)); nia. *)
+    (*}*)
+    (*specialize (fold_right_time_bound_env H4 H5) as (f & G1 & G2 & G3).*)
+    (*exists (fun n => f (n + 2)). *)
+    (*split.*)
+    (*- intros. rewrite G1 with (env := tt). now rewrite <- size_unit_enc. *)
+    (*- split; smpl_inO. apply inOPoly_comp; smpl_inO. *)
+  (*Qed. *)
 End noEnv.
 
